hax-lib/proof-libs/lean/Hax/CoreModels.lean
@@ -1,7 +1,7 @@
 
 -- Experimental lean backend for Hax
 -- The Hax prelude library can be found in hax/proof-libs/lean
-import Hax
+import Hax.Core
 import Std.Tactic.Do
 import Std.Do.Triple
 import Std.Tactic.Do.Syntax
