hax-lib/proof-libs/lean/Hax/MissingCoreModels.lean
@@ -1,0 +1,94 @@
+import Hax.CoreModels
+
+set_option mvcgen.warning false
+open Rust_primitives.Hax
+open Core.Ops
+open Std.Do
+
+namespace Core_models.Result
+
+def Impl.unwrap
+  (T : Type) (E : Type) (self : (Result T E))
+  : RustM T
+  := do
+  match self with
+    | (Result.Ok t) => (pure t)
+    | (Result.Err _)
+      => (Core_models.Panicking.Internal.panic T Rust_primitives.Hax.Tuple0.mk)
+
+@[spec]
+theorem Impl.unwrap.spec {α β} (x: Result α β) v :
+  x = Result.Ok v →
+  ⦃ ⌜ True ⌝ ⦄
+  (Impl.unwrap α β x)
+  ⦃ ⇓ r => ⌜ r = v ⌝ ⦄
+  := by
+  intros
+  mvcgen [Impl.unwrap] <;> try grind
+
+end Core_models.Result
+
+namespace Core_models.Convert
+
+@[reducible] instance {α : Type} {n : Nat} : TryInto.AssociatedTypes (RustSlice α) (RustArray α n) where
+  Error := Core_models.Array.TryFromSliceError
+
+instance {α : Type} {n : Nat} : TryInto (RustSlice α) (RustArray α n) where
+  try_into a :=
+   pure (
+     if h: a.size = n then
+       Core_models.Result.Result.Ok (a.toVector.cast h)
+     else
+       .Err Core_models.Array.TryFromSliceError.array.TryFromSliceError
+     )
+
+@[spec]
+theorem TryInto.try_into.spec {α : Type} {n: Nat} (a: RustSlice α) :
+  (h: a.size = n) →
+  ⦃ ⌜ True ⌝ ⦄
+  (TryInto.try_into (RustSlice α) (RustArray α n) a )
+  ⦃ ⇓ r => ⌜ r = .Ok (a.toVector.cast h) ⌝ ⦄ := by
+  intro h
+  mvcgen [TryInto.try_into]
+  grind
+
+end Core_models.Convert
+
+
+namespace Core_models.Ops.Function
+
+instance {α β} : FnOnce.AssociatedTypes (α → RustM β) α where
+  Output := β
+
+instance {α β} : FnOnce.AssociatedTypes (α → RustM β) (Tuple1 α) where
+  Output := β
+
+instance {α β γ} : FnOnce.AssociatedTypes (α → β → RustM γ) (Tuple2 α β) where
+  Output := γ
+
+instance {α β} : FnOnce (α → RustM β) α where
+  call_once f x := f x
+
+instance {α β} : FnOnce (α → RustM β) (Tuple1 α) where
+  call_once f x := f x._0
+
+instance {α β γ : Type} : FnOnce (α → β → RustM γ) (Tuple2 α β) where
+  call_once f x := f x._0 x._1
+
+class Fn (Self Args : Type) where
+  [_constr1 : outParam (FnOnce.AssociatedTypes Self Args)]
+  [_constr2 : (FnOnce Self Args)]
+  call (Self Args) : Self -> Args -> RustM (FnOnce.Output Self Args)
+
+instance {α β} [FnOnce.AssociatedTypes (α → RustM β) α] [FnOnce (α → RustM β) α] : Fn (α → RustM β) α where
+  call f x := FnOnce.call_once _ _ f x
+
+instance {α β} [FnOnce.AssociatedTypes (α → RustM β) (Tuple1 α)] [FnOnce (α → RustM β) (Tuple1 α)] :
+    Fn (α → RustM β) (Tuple1 α) where
+  call f x := FnOnce.call_once _ _ f x
+
+instance {α β γ} [FnOnce.AssociatedTypes (α → β → RustM γ) (Tuple2 α β)] [FnOnce (α → β → RustM γ) (Tuple2 α β)] :
+    Fn (α → β → RustM γ) (Tuple2 α β) where
+  call f x := FnOnce.call_once _ _ f x
+
+end Core_models.Ops.Function
